src/proofs/no_slashable_attestations/supporting_lemmas/dv_next_preserves_ind_inv/ind_inv_dv_next.dfy
@@ -16,7 +16,6 @@ include "invs_dv_next_2.dfy"
 include "invs_dv_next_3.dfy"
 include "invs_dv_next_4.dfy"
 include "invs_dv_next_5.dfy"
-include "invs_dv_next_6.dfy"
 
 include "../inv.dfy"
 include "../ind_inv.dfy"
@@ -33,15 +32,14 @@ module Ind_Inv_DV_Next
     import opened DV
     import opened Att_Ind_Inv_With_Empty_Init_Att_Slashing_DB
     import opened Att_Inv_With_Empty_Initial_Attestation_Slashing_DB
-    import opened Invs_DV_Next_3
-    import opened Invs_DV_Next_4
-    import opened Fnc_Invs_1
     import opened Helper_Sets_Lemmas
     import opened Invs_DV_Next_1
-    import opened Proofs_Intermediate_Steps
     import opened Invs_DV_Next_2
+    import opened Invs_DV_Next_3
+    import opened Invs_DV_Next_4
     import opened Invs_DV_Next_5
-    import opened Invs_DV_Next_6
+    import opened Proofs_Intermediate_Steps
+    
 
     lemma lem_ind_inv_dv_next_invs_group_1(dv: DVState, e: DV.Event, dv': DVState)       
     requires DV.NextEventPreCond(dv, e)
@@ -52,8 +50,6 @@ module Ind_Inv_DV_Next
         lem_inv_quorum_constraints_dv_next(dv, e, dv');
         lem_inv_unchanged_honesty_dv_next(dv, e, dv');
         lem_inv_only_dv_construct_signed_attestation_signature_dv_next(dv, e, dv');
-        lem_inv_queued_att_duty_is_dvn_seq_of_att_duty_dv_next(dv, e, dv');
-        lem_inv_queued_att_duty_is_rcvd_duty_dv_next(dv, e, dv');
         lem_inv_current_att_duty_is_rcvd_duty_dv_next(dv, e, dv');
         lem_inv_latest_served_duty_is_rcvd_duty_dv_next(dv, e, dv');        
     }
@@ -74,17 +70,6 @@ module Ind_Inv_DV_Next
     requires DV.NextEventPreCond(dv, e)
     requires DV.NextEvent(dv, e, dv')  
     requires ind_inv(dv)
-    ensures invs_group_3(dv')
-    {
-        lem_inv_no_queued_att_duty_if_latest_served_att_duty_is_none_dv_next(dv, e, dv');
-        lem_inv_strictly_increasing_queue_of_att_duties_dv_next(dv, e, dv');
-        lem_inv_queued_att_duty_is_higher_than_latest_served_att_duty_dv_next(dv, e, dv');
-    }
-
-    lemma lem_ind_inv_dv_next_invs_group_4(dv: DVState, e: DV.Event, dv': DVState)       
-    requires DV.NextEventPreCond(dv, e)
-    requires DV.NextEvent(dv, e, dv')  
-    requires ind_inv(dv)
     ensures invs_group_4(dv')
     {
         lem_inv_no_duplicated_att_duties_dv_next(dv, e, dv');
@@ -92,7 +77,7 @@ module Ind_Inv_DV_Next
         lem_inv_no_active_consensus_instance_before_receiving_an_att_duty_dv_next(dv, e, dv');                        
     }
 
-    lemma lem_ind_inv_dv_next_invs_group_5(dv: DVState, e: DV.Event, dv': DVState)       
+    lemma lem_ind_inv_dv_next_invs_group_4(dv: DVState, e: DV.Event, dv': DVState)       
     requires DV.NextEventPreCond(dv, e)
     requires DV.NextEvent(dv, e, dv')  
     requires ind_inv(dv)
@@ -104,7 +89,7 @@ module Ind_Inv_DV_Next
     }
 
 
-    lemma lem_ind_inv_dv_next_invs_group_6(dv: DVState, e: DV.Event, dv': DVState)       
+    lemma lem_ind_inv_dv_next_invs_group_5(dv: DVState, e: DV.Event, dv': DVState)       
     requires DV.NextEventPreCond(dv, e)
     requires DV.NextEvent(dv, e, dv')  
     requires ind_inv(dv)
@@ -115,25 +100,22 @@ module Ind_Inv_DV_Next
         lem_inv_validity_pred_for_slot_k_is_stored_in_att_slashing_db_hist_k_dv_next(dv, e, dv');          
     }
 
+    lemma lem_ind_inv_dv_next_invs_group_6(dv: DVState, e: DV.Event, dv': DVState)       
+    requires DV.NextEventPreCond(dv, e)
+    requires DV.NextEvent(dv, e, dv')  
+    requires ind_inv(dv)
+    ensures invs_group_6(dv')
+    {       
+        lem_inv_every_db_in_att_slashing_db_hist_is_subset_of_att_slashing_db_dv_next(dv, e, dv');  
+        lem_inv_active_attn_consensus_instances_are_tracked_in_att_slashing_db_hist_dv_next(dv, e, dv');  
+        lem_inv_construct_signed_attestation_signature_assumptions_helper_dv_next(dv, e, dv');  
+    }
+
     lemma lem_ind_inv_dv_next_invs_group_7(dv: DVState, e: DV.Event, dv': DVState)       
     requires DV.NextEventPreCond(dv, e)
     requires DV.NextEvent(dv, e, dv')  
     requires ind_inv(dv)
     ensures invs_group_7(dv')
-    {       
-        lem_inv_every_db_in_att_slashing_db_hist_is_subset_of_att_slashing_db_dv_next(dv, e, dv');  
-        lem_inv_active_attn_consensus_instances_are_tracked_in_att_slashing_db_hist_dv_next(dv, e, dv');  
-        lem_inv_construct_signed_attestation_signature_assumptions_helper_dv_next(dv, e, dv');  
-        // lem_inv_all_in_transit_messages_were_sent_dv_next(dv, e, dv');  
-        // lem_inv_rcvd_attn_shares_are_from_sent_messages_dv_next(dv, e, dv');  
-        // Invs_DV_Next_5.lem_inv_33(dv, e, dv');
-    }
-
-    lemma lem_ind_inv_dv_next_invs_group_8(dv: DVState, e: DV.Event, dv': DVState)       
-    requires DV.NextEventPreCond(dv, e)
-    requires DV.NextEvent(dv, e, dv')  
-    requires ind_inv(dv)
-    ensures invs_group_8(dv')
     {               
         lem_inv_all_in_transit_messages_were_sent_dv_next(dv, e, dv');  
         lem_inv_rcvd_attn_shares_are_from_sent_messages_dv_next(dv, e, dv');  
@@ -143,22 +125,18 @@ module Ind_Inv_DV_Next
 
     lemma lem_ind_inv_implies_intermediate_steps_helper_1(dv: DVState)
     requires ind_inv(dv)
-    ensures concl_next_att_duty_is_higher_than_current_att_duty(dv)
-    ensures concl_next_att_duty_is_higher_than_latest_served_att_duty(dv)
-    ensures concl_future_att_duty_is_higher_than_rcvd_att_duty(dv)
-    ensures concl_future_att_duty_is_higher_than_queued_att_duty(dv)
-    ensures concl_slot_of_active_consensus_instance_is_lower_than_slot_of_queued_att_duty(dv)    
+    ensures inv_next_att_duty_is_higher_than_current_att_duty(dv)
+    ensures inv_next_att_duty_is_higher_than_latest_served_att_duty(dv)
+    ensures inv_future_att_duty_is_higher_than_rcvd_att_duty(dv)
     {    
-        lem_concl_next_att_duty_is_higher_than_current_att_duty_ind_inv(dv);
-        lem_concl_next_att_duty_is_higher_than_latest_served_att_duty_ind_inv(dv);
-        lem_concl_future_att_duty_is_higher_than_rcvd_att_duty_ind_inv(dv);
-        lem_concl_future_att_duty_is_higher_than_queued_att_duty_ind_inv(dv);
-        lem_concl_slot_of_active_consensus_instance_is_lower_than_slot_of_queued_att_duty_ind_inv(dv);  
+        lem_inv_next_att_duty_is_higher_than_current_att_duty_ind_inv(dv);
+        lem_inv_next_att_duty_is_higher_than_latest_served_att_duty_ind_inv(dv);
+        lem_inv_future_att_duty_is_higher_than_rcvd_att_duty_ind_inv(dv);
     }
 
     lemma lem_ind_inv_implies_intermediate_steps_helper_2(dv: DVState)
     requires ind_inv(dv)  
-    ensures inv_queued_att_duty_is_rcvd_duty0(dv)
+    ensures inv_sent_vp_is_based_on_existing_slashing_db_and_rcvd_att_duty(dv)
     ensures inv_queued_att_duty_is_rcvd_duty1(dv)   
     ensures same_honest_nodes_in_dv_and_ci(dv)    
     ensures construct_signed_attestation_signature_assumptions_helper(
@@ -166,7 +144,7 @@ module Ind_Inv_DV_Next
                 dv.dv_pubkey,
                 dv.all_nodes)  
     {    
-        lem_inv_queued_att_duty_is_rcvd_duty0_ind_inv(dv);
+        lem_inv_sent_vp_is_based_on_existing_slashing_db_and_rcvd_att_duty_ind_inv(dv);
         lem_inv_queued_att_duty_is_rcvd_duty1_ind_inv(dv);
         lem_inv_queued_att_duty_is_rcvd_duty3_ind_inv(dv);      
         lem_construct_signed_attestation_signature_assumptions_helper(dv);       
@@ -174,24 +152,19 @@ module Ind_Inv_DV_Next
 
     lemma lem_ind_inv_implies_intermediate_steps_helper_3(dv: DVState)
     requires ind_inv(dv)  
-    ensures inv_head_attetation_duty_queue_higher_than_latest_attestation_duty(dv)  
     ensures is_sequence_attestation_duties_to_be_served_orderd(dv)
-    ensures inv_attestation_duty_queue_is_ordered(dv)
     ensures inv_active_attestation_consensus_instances_keys_is_subset_of_att_slashing_db_hist(dv)
-    ensures pred_inv_current_latest_attestation_duty_match(dv)
+    ensures inv_current_latest_attestation_duty_match(dv)
     ensures pred_rcvd_attestation_shares_is_in_all_messages_sent(dv)
     {    
-        lem_inv_head_attetation_duty_queue_higher_than_latest_attestation_duty(dv);
-        lem_inv_attestation_duty_queue_is_ordered(dv);
         lem_inv_active_attestation_consensus_instances_keys_is_subset_of_att_slashing_db_hist(dv);
-        lem_pred_inv_current_latest_attestation_duty_match(dv);
+        lem_inv_current_latest_attestation_duty_match(dv);
         lem_inv_rcvd_attn_shares_are_from_sent_messages_pred_rcvd_attestation_shares_is_in_all_messages_sent(dv);
     }
 
     lemma lem_ind_inv_implies_intermediate_steps_helper_4(dv: DVState)
     requires ind_inv(dv)  
-    ensures lem_inv_db_of_validity_predicate_contains_all_previous_decided_values_precond(dv)
-    ensures lem_concl_exists_honest_dvc_that_sent_att_share_for_submitted_att_new_precond(dv)    
+    ensures lem_inv_exists_honest_dvc_that_sent_att_share_for_submitted_att_new_precond(dv)    
     {   
         lem_ind_inv_implies_intermediate_steps_helper_1(dv);
         lem_ind_inv_implies_intermediate_steps_helper_2(dv);
@@ -200,26 +173,21 @@ module Ind_Inv_DV_Next
 
     lemma lem_ind_inv_implies_intermediate_steps(dv: DVState)
     requires ind_inv(dv)
-    ensures concl_next_att_duty_is_higher_than_current_att_duty(dv)
-    ensures concl_next_att_duty_is_higher_than_latest_served_att_duty(dv)
-    ensures concl_future_att_duty_is_higher_than_rcvd_att_duty(dv)
-    ensures concl_future_att_duty_is_higher_than_queued_att_duty(dv)
-    ensures concl_slot_of_active_consensus_instance_is_lower_than_slot_of_queued_att_duty(dv)    
-    ensures inv_queued_att_duty_is_rcvd_duty0(dv)
+    ensures inv_next_att_duty_is_higher_than_current_att_duty(dv)
+    ensures inv_next_att_duty_is_higher_than_latest_served_att_duty(dv)
+    ensures inv_future_att_duty_is_higher_than_rcvd_att_duty(dv)
+    ensures inv_sent_vp_is_based_on_existing_slashing_db_and_rcvd_att_duty(dv)
     ensures inv_queued_att_duty_is_rcvd_duty1(dv)   
     ensures same_honest_nodes_in_dv_and_ci(dv)    
     ensures construct_signed_attestation_signature_assumptions_helper(
                 dv.construct_signed_attestation_signature,
                 dv.dv_pubkey,
                 dv.all_nodes)  
-    ensures inv_head_attetation_duty_queue_higher_than_latest_attestation_duty(dv)   
     ensures is_sequence_attestation_duties_to_be_served_orderd(dv)     
-    ensures inv_attestation_duty_queue_is_ordered(dv)
     ensures inv_active_attestation_consensus_instances_keys_is_subset_of_att_slashing_db_hist(dv)
-    ensures pred_inv_current_latest_attestation_duty_match(dv)
+    ensures inv_current_latest_attestation_duty_match(dv)
     ensures pred_rcvd_attestation_shares_is_in_all_messages_sent(dv)
-    ensures lem_inv_db_of_validity_predicate_contains_all_previous_decided_values_precond(dv)
-    ensures lem_concl_exists_honest_dvc_that_sent_att_share_for_submitted_att_new_precond(dv)
+    ensures lem_inv_exists_honest_dvc_that_sent_att_share_for_submitted_att_new_precond(dv)
     {   
         lem_ind_inv_implies_intermediate_steps_helper_1(dv); 
         lem_ind_inv_implies_intermediate_steps_helper_2(dv);
@@ -256,11 +224,11 @@ module Ind_Inv_DV_Next
         assert inv_all_validity_predicates_are_stored_in_att_slashing_db_hist(dv');
     }
 
-    lemma lem_ind_inv_dv_next_inv_concl_exists_honest_dvc_that_sent_att_share_for_submitted_att(dv: DVState, e: DV.Event, dv': DVState)       
+    lemma lem_ind_inv_dv_next_inv_exists_honest_dvc_that_sent_att_share_for_submitted_att(dv: DVState, e: DV.Event, dv': DVState)       
     requires DV.NextEventPreCond(dv, e)
     requires DV.NextEvent(dv, e, dv')  
     requires ind_inv(dv)
-    ensures concl_exists_honest_dvc_that_sent_att_share_for_submitted_att(dv')
+    ensures inv_exists_honest_dvc_that_sent_att_share_for_submitted_att(dv')
     {
         lem_ind_inv_implies_intermediate_steps(dv);
         assert construct_signed_attestation_signature_assumptions_helper(
@@ -275,7 +243,7 @@ module Ind_Inv_DV_Next
         assert pred_rcvd_attestation_shares_is_in_all_messages_sent(dv);
 
         assert  && DV.NextEvent(dv, e, dv')
-                && concl_exists_honest_dvc_that_sent_att_share_for_submitted_att(dv)
+                && inv_exists_honest_dvc_that_sent_att_share_for_submitted_att(dv)
                 && construct_signed_attestation_signature_assumptions_helper(
                     dv.construct_signed_attestation_signature,
                     dv.dv_pubkey,
@@ -288,8 +256,8 @@ module Ind_Inv_DV_Next
                 ;
 
         
-        lem_concl_exists_honest_dvc_that_sent_att_share_for_submitted_att(dv, e, dv');
-        assert concl_exists_honest_dvc_that_sent_att_share_for_submitted_att(dv');
+        lem_inv_exists_honest_dvc_that_sent_att_share_for_submitted_att(dv, e, dv');
+        assert inv_exists_honest_dvc_that_sent_att_share_for_submitted_att(dv');
     }
 
     lemma lem_ind_inv_dv_next_inv_decided_value_of_consensus_instance_is_decided_by_quorum(dv: DVState, e: DV.Event, dv': DVState)       
@@ -329,14 +297,14 @@ module Ind_Inv_DV_Next
     }
 
     
-    lemma lem_ind_inv_dv_next_invs_group_9(dv: DVState, e: DV.Event, dv': DVState)       
+    lemma lem_ind_inv_dv_next_invs_group_8(dv: DVState, e: DV.Event, dv': DVState)       
     requires DV.NextEventPreCond(dv, e)
     requires DV.NextEvent(dv, e, dv')  
     requires ind_inv(dv)
-    ensures invs_group_9(dv')
+    ensures invs_group_8(dv')
     {
         lem_ind_inv_dv_next_inv_all_validity_predicates_are_stored_in_att_slashing_db_hist(dv, e, dv');  
-        lem_ind_inv_dv_next_inv_concl_exists_honest_dvc_that_sent_att_share_for_submitted_att(dv, e, dv');             
+        lem_ind_inv_dv_next_inv_exists_honest_dvc_that_sent_att_share_for_submitted_att(dv, e, dv');             
         lem_ind_inv_dv_next_inv_decided_value_of_consensus_instance_is_decided_by_quorum(dv, e, dv');       
         lem_ind_inv_dv_next_inv_sent_validity_predicate_is_based_on_rcvd_att_duty_and_slashing_db_for_dv(dv, e, dv');  
         lem_ind_inv_dv_next_inv_sent_validity_predicate_is_based_on_rcvd_att_duty_and_slashing_db(dv, e, dv');   
@@ -372,11 +340,11 @@ module Ind_Inv_DV_Next
         lem_inv_exists_att_duty_in_dv_seq_of_att_duty_for_every_slot_in_att_slashing_db_hist(dv, e, dv');
     }
 
-    lemma lem_ind_inv_dv_next_invs_group_10(dv: DVState, e: DV.Event, dv': DVState)       
+    lemma lem_ind_inv_dv_next_invs_group_9(dv: DVState, e: DV.Event, dv': DVState)       
     requires DV.NextEventPreCond(dv, e)
     requires DV.NextEvent(dv, e, dv')  
     requires ind_inv(dv)
-    ensures invs_group_10(dv')
+    ensures invs_group_9(dv')
     {
         lem_inv_decided_value_of_consensus_instance_of_slot_k_is_for_slot_k(dv, e, dv');
         lem_ind_inv_dv_next_invNetwork(dv, e, dv');
@@ -384,19 +352,37 @@ module Ind_Inv_DV_Next
         lem_inv_attestation_shares_to_broadcast_are_sent_messages_inv_attestation_shares_to_broadcast_is_a_subset_of_all_messages_sent(dv');
     }
 
-    lemma lem_inv_db_of_validity_predicate_contains_all_previous_decided_values_ind_inv(
-        dv: DVState,
-        event: DV.Event,
-        dv': DVState
-    )
-    requires NextEvent.requires(dv, event, dv')
-    requires NextEvent(dv, event, dv')
+    lemma lem_ind_inv_dv_next_invs_group_10(dv: DVState, e: DV.Event, dv': DVState)       
+    requires DV.NextEventPreCond(dv, e)
+    requires DV.NextEvent(dv, e, dv')  
     requires ind_inv(dv)
-    ensures inv_db_of_validity_predicate_contains_all_previous_decided_values(dv')
+    ensures invs_group_10(dv')
+    {        
+        lem_ind_inv_dv_next_inv_exists_att_duty_in_dv_seq_of_att_duty_for_every_slot_in_att_slashing_db_hist(dv, e, dv');
+        lem_inv_available_latest_attestation_duty_is_from_dv_seq_of_att_duties_new_body_dv_next(dv, e, dv');
+        lem_inv_exists_att_duty_in_dv_seq_of_att_duty_for_every_slot_in_att_slashing_db_hist_a(dv, e, dv');
+        lem_ind_inv_implies_intermediate_steps(dv);
+        lem_inv_data_of_att_share_is_decided_value(dv, e, dv');
+    }
+    
+    lemma lem_ind_inv_dv_next_inv_future_decided_data_of_dvc_is_consistent_with_existing_decision_dv(dv: DVState, e: DV.Event, dv': DVState)       
+    requires DV.NextEventPreCond(dv, e)
+    requires DV.NextEvent(dv, e, dv')  
+    requires ind_inv(dv)
+    ensures inv_future_decided_data_of_dvc_is_consistent_with_existing_decision_dv(dv')
     {
         lem_ind_inv_implies_intermediate_steps_helper_4(dv);
-        assert lem_inv_db_of_validity_predicate_contains_all_previous_decided_values_precond(dv);
-        lem_inv_db_of_validity_predicate_contains_all_previous_decided_values(dv, event, dv');
+        lem_inv_future_decided_data_of_dvc_is_consistent_with_existing_decision_dv(dv, e, dv');
+    }
+
+    lemma lem_ind_inv_dv_next_inv_slot_in_future_decided_data_is_correct(dv: DVState, e: DV.Event, dv': DVState)       
+    requires DV.NextEventPreCond(dv, e)
+    requires DV.NextEvent(dv, e, dv')  
+    requires ind_inv(dv)
+    ensures inv_slot_in_future_decided_data_is_correct(dv')
+    {
+        lem_ind_inv_implies_intermediate_steps_helper_4(dv);
+        lem_inv_slot_in_future_decided_data_is_correct(dv, e, dv');
     }
 
     lemma lem_ind_inv_dv_next_invs_group_11(dv: DVState, e: DV.Event, dv': DVState)       
@@ -404,115 +390,21 @@ module Ind_Inv_DV_Next
     requires DV.NextEvent(dv, e, dv')  
     requires ind_inv(dv)
     ensures invs_group_11(dv')
-    {        
-        lem_ind_inv_dv_next_inv_exists_att_duty_in_dv_seq_of_att_duty_for_every_slot_in_att_slashing_db_hist(dv, e, dv');
-        lem_inv_available_latest_attestation_duty_is_from_dv_seq_of_att_duties_new_body_dv_next(dv, e, dv');
-        lem_inv_exists_att_duty_in_dv_seq_of_att_duty_for_every_slot_in_att_slashing_db_hist_a(dv, e, dv');
-        lem_ind_inv_implies_intermediate_steps(dv);
-        lem_pred_data_of_att_share_is_decided_value(dv, e, dv');
+    {
+        lem_ind_inv_implies_intermediate_steps_helper_4(dv);
+        lem_inv_future_decided_data_of_dvc_is_consistent_with_existing_decision_dv(dv, e, dv');
+        lem_inv_slot_in_future_decided_data_is_correct(dv, e, dv');        
     }
-    
+
     lemma lem_ind_inv_dv_next_invs_group_12(dv: DVState, e: DV.Event, dv': DVState)       
     requires DV.NextEventPreCond(dv, e)
     requires DV.NextEvent(dv, e, dv')  
     requires ind_inv(dv)
     ensures invs_group_12(dv')
-    {        
-        lem_inv_attestation_duty_queue_is_ordered_3(dv, e, dv');
-        lem_inv_attestation_duty_queue_is_ordered_4(dv, e, dv');        
-    }
-
-    lemma lem_ind_inv_dv_next_inv_queued_att_duties_are_from_dv_seq_of_att_duties(dv: DVState, e: DV.Event, dv': DVState)       
-    requires DV.NextEventPreCond(dv, e)
-    requires DV.NextEvent(dv, e, dv')  
-    requires ind_inv(dv)
-    ensures inv_queued_att_duties_are_from_dv_seq_of_att_duties(dv')
     {
         lem_ind_inv_implies_intermediate_steps_helper_4(dv);
-        lem_inv_queued_att_duties_are_from_dv_seq_of_att_duties_dv_next(dv, e, dv');
-    }
-
-    lemma lem_ind_inv_dv_next_inv_inv_decided_values_of_previous_duties_are_known_new(dv: DVState, e: DV.Event, dv': DVState)       
-    requires DV.NextEventPreCond(dv, e)
-    requires DV.NextEvent(dv, e, dv')  
-    requires ind_inv(dv)
-    ensures inv_decided_values_of_previous_duties_are_known_new(dv')
-    {
-        lem_ind_inv_implies_intermediate_steps_helper_4(dv);
-        lem_concl_exists_honest_dvc_that_sent_att_share_for_submitted_att_new(dv, e, dv');
-    }
-
-    lemma lem_ind_inv_dv_next_inv_g_d_a(dv: DVState, e: DV.Event, dv': DVState)       
-    requires DV.NextEventPreCond(dv, e)
-    requires DV.NextEvent(dv, e, dv')  
-    requires ind_inv(dv)
-    ensures inv_g_d_a(dv')
-    {
-        lem_ind_inv_implies_intermediate_steps_helper_4(dv);
-        lem_inv_g_d_a(dv, e, dv');
-    }
-
-    lemma lem_ind_inv_dv_next_inv_g_d_b(dv: DVState, e: DV.Event, dv': DVState)       
-    requires DV.NextEventPreCond(dv, e)
-    requires DV.NextEvent(dv, e, dv')  
-    requires ind_inv(dv)
-    ensures inv_g_d_b(dv')
-    {
-        lem_ind_inv_implies_intermediate_steps_helper_4(dv);
-        lem_inv_g_d_b(dv, e, dv');
-    }
-
-    lemma lem_ind_inv_dv_next_inv_exists_decided_value_for_every_duty_before_queued_duties(dv: DVState, e: DV.Event, dv': DVState)       
-    requires DV.NextEventPreCond(dv, e)
-    requires DV.NextEvent(dv, e, dv')  
-    requires ind_inv(dv)
-    ensures inv_exists_decided_value_for_every_duty_before_queued_duties(dv')
-    {
-        lem_ind_inv_implies_intermediate_steps_helper_4(dv);
-        lem_inv_exists_decided_value_for_every_duty_before_queued_duties(dv, e, dv');
-    }
-
-
-
-    lemma lem_ind_inv_dv_next_invs_group_13(dv: DVState, e: DV.Event, dv': DVState)       
-    requires DV.NextEventPreCond(dv, e)
-    requires DV.NextEvent(dv, e, dv')  
-    requires ind_inv(dv)
-    ensures invs_group_13(dv')
-    {
-        lem_ind_inv_implies_intermediate_steps_helper_4(dv);
-        
-        lem_inv_queued_att_duties_are_from_dv_seq_of_att_duties_dv_next(dv, e, dv');
-        lem_concl_exists_honest_dvc_that_sent_att_share_for_submitted_att_new(dv, e, dv');
-        lem_inv_g_d_a(dv, e, dv');
-        lem_inv_g_d_b(dv, e, dv');        
-        lem_inv_exists_decided_value_for_every_duty_before_queued_duties(dv, e, dv');
-    }
-
-    lemma lem_ind_inv_dv_next_invs_group_14(dv: DVState, e: DV.Event, dv': DVState)       
-    requires DV.NextEventPreCond(dv, e)
-    requires DV.NextEvent(dv, e, dv')  
-    requires ind_inv(dv)
-    ensures invs_group_14(dv')
-    {
-        lem_ind_inv_implies_intermediate_steps_helper_4(dv);
-
-        lem_inv_g_a_iii(dv, e, dv');
-        lem_inv_g_a_iv_a(dv, e, dv');
-        lem_inv_db_of_validity_predicate_contains_all_previous_decided_values(dv, e, dv');        
-    }
-
-    lemma lem_ind_inv_dv_next_invs_group_15(dv: DVState, e: DV.Event, dv': DVState)       
-    requires DV.NextEventPreCond(dv, e)
-    requires DV.NextEvent(dv, e, dv')  
-    requires ind_inv(dv)
-    ensures invs_group_15(dv')
-    {
-        lem_ind_inv_implies_intermediate_steps_helper_4(dv);
-
         lem_inv_sent_validity_predicate_only_for_slots_stored_in_att_slashing_db_hist(dv, e, dv');
         lem_inv_all_validity_predicates_are_stored_in_att_slashing_db_hist(dv, e, dv');
-        lem_inv_no_instance_has_been_started_for_duties_in_attestation_duty_queue_next_honest(dv, e, dv');       
     }
     
     lemma lem_ind_inv_dv_next_ind_inv_helper_1(dv: DVState, e: DV.Event, dv': DVState)       
@@ -560,19 +452,6 @@ module Ind_Inv_DV_Next
         lem_ind_inv_dv_next_invs_group_12(dv, e, dv');                              
     }
 
-    lemma lem_ind_inv_dv_next_ind_inv_helper_4(dv: DVState, e: DV.Event, dv': DVState)       
-    requires DV.NextEventPreCond(dv, e)
-    requires DV.NextEvent(dv, e, dv')  
-    requires ind_inv(dv)    
-    ensures invs_group_13(dv')
-    ensures invs_group_14(dv')
-    ensures invs_group_15(dv')
-    {                 
-        lem_ind_inv_dv_next_invs_group_13(dv, e, dv');            
-        lem_ind_inv_dv_next_invs_group_14(dv, e, dv');            
-        lem_ind_inv_dv_next_invs_group_15(dv, e, dv');            
-    }
-
     lemma lem_ind_inv_dv_next_ind_inv_helper_a(dv: DVState, e: DV.Event, dv': DVState)       
     requires DV.NextEventPreCond(dv, e)
     requires DV.NextEvent(dv, e, dv')  
@@ -598,12 +477,8 @@ module Ind_Inv_DV_Next
     ensures invs_group_10(dv')    
     ensures invs_group_11(dv')    
     ensures invs_group_12(dv')    
-    ensures invs_group_13(dv')    
-    ensures invs_group_14(dv')  
-    ensures invs_group_15(dv')  
     {
         lem_ind_inv_dv_next_ind_inv_helper_3(dv, e, dv');     
-        lem_ind_inv_dv_next_ind_inv_helper_4(dv, e, dv');            
     }
 
     lemma lem_ind_inv_dv_next_ind_inv_helper(dv: DVState, e: DV.Event, dv': DVState)       
@@ -622,9 +497,6 @@ module Ind_Inv_DV_Next
     ensures invs_group_10(dv')    
     ensures invs_group_11(dv')    
     ensures invs_group_12(dv')    
-    ensures invs_group_13(dv')    
-    ensures invs_group_14(dv')    
-    ensures invs_group_15(dv')    
     {   
         lem_ind_inv_dv_next_ind_inv_helper_a(dv, e, dv');
         lem_ind_inv_dv_next_ind_inv_helper_b(dv, e, dv');                
@@ -657,13 +529,10 @@ module Ind_Inv_DV_Next
     lemma lem_NextPreCond(
         s: DVState
     )
-    requires inv_no_instance_has_been_started_for_duties_in_attestation_duty_queue(s);
     requires is_sequence_attestation_duties_to_be_served_orderd(s)
-    requires inv_queued_att_duties_are_from_dv_seq_of_att_duties(s)
     requires inv_latest_attestation_duty_is_from_dv_seq_of_att_duties(s)
     requires inv_slot_of_active_consensus_instance_is_not_higher_than_slot_of_latest_served_att_duty(s)
     requires inv_no_active_consensus_instance_before_receiving_an_att_duty(s)
-    requires inv_head_attetation_duty_queue_higher_than_latest_attestation_duty(s)   
     ensures  NextPreCond(s)                
     {
         forall event | validEvent(s, event)
