src/proofs/no_slashable_attestations/supporting_lemmas/ind_inv.dfy
@@ -29,10 +29,7 @@ module Att_Ind_Inv_With_Empty_Init_Att_Slashing_DB
         && invs_group_9(dv)
         && invs_group_10(dv)
         && invs_group_11(dv)
-        && invs_group_12(dv)
-        && invs_group_13(dv)
-        && invs_group_14(dv)
-        && invs_group_15(dv)        
+        && invs_group_12(dv)        
     }
 
     predicate invs_group_1(dv: DVState)       
@@ -41,7 +38,6 @@ module Att_Ind_Inv_With_Empty_Init_Att_Slashing_DB
         &&  inv_unchanged_honesty(dv)
         &&  inv_only_dv_construct_signed_attestation_signature(dv)
         &&  inv_queued_att_duty_is_dvn_seq_of_att_duty(dv)
-        // &&  inv_queued_att_duty_is_rcvd_duty(dv)
         &&  inv_current_att_duty_is_rcvd_duty(dv)
         &&  inv_latest_served_duty_is_rcvd_duty(dv)
     }
@@ -56,58 +52,50 @@ module Att_Ind_Inv_With_Empty_Init_Att_Slashing_DB
 
     predicate invs_group_3(dv: DVState)       
     {        
-        // &&  inv_no_queued_att_duty_if_latest_served_att_duty_is_none(dv)  
-        // &&  inv_strictly_increasing_queue_of_att_duties(dv)  
-        // &&  inv_queued_att_duty_is_higher_than_latest_served_att_duty(dv)  
-        && true
-    }
-
-    predicate invs_group_4(dv: DVState)       
-    {        
         &&  inv_no_duplicated_att_duties(dv)           
         &&  inv_every_att_duty_before_dvn_att_index_was_delivered(dv) 
         &&  inv_no_active_consensus_instance_before_receiving_an_att_duty(dv)              
     }
 
-    predicate invs_group_5(dv: DVState)       
+    predicate invs_group_4(dv: DVState)       
     {        
         &&  inv_slot_of_active_consensus_instance_is_not_higher_than_slot_of_latest_served_att_duty(dv)  
         &&  inv_consensus_instance_only_for_slot_in_which_dvc_has_rcvd_att_duty(dv)          
         &&  inv_consensus_instances_only_for_rcvd_duties(dv)  
     }
 
-    predicate invs_group_6(dv: DVState)       
+    predicate invs_group_5(dv: DVState)       
     {                
         &&  inv_att_slashing_db_hist_keeps_track_of_only_rcvd_att_duties(dv)  
         &&  inv_exists_db_in_att_slashing_db_hist_for_every_validity_pred(dv)  
         &&  inv_validity_pred_for_slot_k_is_stored_in_att_slashing_db_hist_k(dv)          
     }
 
-    predicate invs_group_7(dv: DVState)       
+    predicate invs_group_6(dv: DVState)       
     {                
         &&  inv_every_db_in_att_slashing_db_hist_is_subset_of_att_slashing_db(dv)  
         &&  inv_active_attn_consensus_instances_are_tracked_in_att_slashing_db_hist(dv)
         &&  inv_construct_signed_attestation_signature_assumptions_helper(dv)        
     }
 
-    predicate invs_group_8(dv: DVState)       
+    predicate invs_group_7(dv: DVState)       
     {                
         &&  inv_all_in_transit_messages_were_sent(dv)
         &&  inv_rcvd_attn_shares_are_from_sent_messages(dv)
         &&  inv_sent_validity_predicate_only_for_slots_stored_in_att_slashing_db_hist_helper(dv)
     }
     
-    predicate invs_group_9(dv: DVState)       
+    predicate invs_group_8(dv: DVState)       
     {                
         && inv_all_validity_predicates_are_stored_in_att_slashing_db_hist(dv)
-        && concl_exists_honest_dvc_that_sent_att_share_for_submitted_att(dv) 
+        && inv_exists_honest_dvc_that_sent_att_share_for_submitted_att(dv) 
         && inv_decided_value_of_consensus_instance_is_decided_by_quorum(dv)    
         && inv_sent_validity_predicate_is_based_on_rcvd_att_duty_and_slashing_db_for_dv(dv)
         && inv_sent_validity_predicate_is_based_on_rcvd_att_duty_and_slashing_db(dv)
         
     }
 
-    predicate invs_group_10(dv: DVState)       
+    predicate invs_group_9(dv: DVState)       
     {                    
         && inv_decided_value_of_consensus_instance_of_slot_k_is_for_slot_k(dv) 
         && invNetwork(dv)
@@ -115,38 +103,21 @@ module Att_Ind_Inv_With_Empty_Init_Att_Slashing_DB
         && inv_attestation_shares_to_broadcast_is_a_subset_of_all_messages_sent(dv)
     }
 
-    predicate invs_group_11(dv: DVState)       
+    predicate invs_group_10(dv: DVState)       
     {                
         && inv_exists_att_duty_in_dv_seq_of_att_duty_for_every_slot_in_att_slashing_db_hist(dv)        
         && inv_latest_attestation_duty_is_from_dv_seq_of_att_duties(dv)
         && inv_exists_att_duty_in_dv_seq_of_att_duty_for_every_slot_in_att_slashing_db_hist_a(dv)        
-        && pred_data_of_att_share_is_decided_value(dv)                     
+        && inv_data_of_att_share_is_decided_value(dv)                     
+    }
+    
+    predicate invs_group_11(dv: DVState)       
+    {                
+        && inv_future_decided_data_of_dvc_is_consistent_with_existing_decision_dv(dv)
+        && inv_slot_in_future_decided_data_is_correct(dv)  
     }
     
     predicate invs_group_12(dv: DVState)       
-    {
-        // && inv_attestation_duty_queue_is_ordered_3(dv)
-        // && inv_attestation_duty_queue_is_ordered_4(dv)
-        && true
-    }
-
-    predicate invs_group_13(dv: DVState)       
-    {                
-        // && inv_queued_att_duties_are_from_dv_seq_of_att_duties(dv)    
-        && inv_decided_values_of_previous_duties_are_known_new(dv)    
-        && inv_g_d_a(dv)
-        && inv_g_d_b(dv)  
-        // && inv_exists_decided_value_for_every_duty_before_queued_duties(dv)        
-    }
-    
-    predicate invs_group_14(dv: DVState)       
-    {                
-        // && inv_g_a_iii(dv)
-        // && inv_g_a_iv_a(dv)
-        && inv_db_of_validity_predicate_contains_all_previous_decided_values(dv)        
-    }
-
-    predicate invs_group_15(dv: DVState)       
     {                
         && inv_sent_validity_predicate_only_for_slots_stored_in_att_slashing_db_hist(dv)
         && inv_all_validity_predicates_are_stored_in_att_slashing_db_hist(dv)
