src/proofs/no_slashable_attestations/supporting_lemmas/init_implies_ind_inv/init_implies_ind_inv.dfy
@@ -28,19 +28,17 @@ module Ind_Inv_DV_Init
                 && invs_group_3(dv)                
                 && invs_group_4(dv)
                 && invs_group_5(dv)   
-                && invs_group_6(dv)                
-                && invs_group_7(dv)
-                && invs_group_8(dv)                
+                && invs_group_6(dv)                     
         ;
 
         assert  DV.Init(dv, {})    
                 ==>
+                && invs_group_7(dv)
+                && invs_group_8(dv)           
                 && invs_group_9(dv)
                 && invs_group_10(dv)
                 && invs_group_11(dv)
                 && invs_group_12(dv)
-                && invs_group_13(dv)
-                && invs_group_14(dv)
-                ;
+        ;
     }  
 }
